Add most typing rules

linear_semtype.v
@@ -4,10 +4,10 @@ Definition TEx (t : tag) (v : val) : sepProp := Ex n, @[ v = VNat n ].
 
 Definition ty := val -> sepProp.
 
+Definition TMoved : ty := fun v => EMP.
 Definition TUnit : ty := fun v => @[ v = VUnit ].
 Definition TNat : ty := fun v => Ex n, @[ v = VNat n ].
 Definition TBool : ty := fun v => Ex b, @[ v = VBool b ].
-Definition TMoved : ty := fun v => EMP.
 
 Definition TRef (A : ty) : ty := fun v =>
   Ex l w, @[ v = VRef l ] ** l ~> w ** A w.
@@ -75,8 +75,12 @@ Definition subty (A1 A2 : ty) : Prop :=
 Definition subctx (Gamma1 Gamma2 : ty_ctx) : Prop :=
   forall vs, ctx_typed Gamma1 vs |~ ctx_typed Gamma2 vs.
 
+Definition bin_op_typed (op : bin_op) (A1 A2 B : ty) : Prop :=
+  forall v1 v2,
+    A1 v1 ** A2 v2 |~ Ex v, @[ eval_bin_op op v1 v2 = Some v ] ** B v.
+
 (* ########################################################################## *)
-(** * Helper lemmas *)
+(** * Helper lemmas and tactics *)
 (* ########################################################################## *)
 
 Lemma subst_map_empty e :
@@ -117,9 +121,41 @@ Proof.
   by rewrite StringMap.delete_empty, subst_map_empty.
 Qed.
 
-(* ########################################################################## *)
-(** * Semantic typing rules *)
-(* ########################################################################## *)
+Lemma PlusOp_typed :
+  bin_op_typed PlusOp TNat TNat TNat.
+Proof.
+  iIntros (v1 v2) "[[%n1 ->] [%n2 ->]]"; simpl; eauto.
+Qed.
+
+Lemma MinusOp_typed :
+  bin_op_typed MinusOp TNat TNat TNat.
+Proof.
+  iIntros (v1 v2) "[[%n1 ->] [%n2 ->]]"; simpl; eauto.
+Qed.
+
+Lemma LeOp_typed :
+  bin_op_typed LeOp TNat TNat TBool.
+Proof.
+  iIntros (v1 v2) "[[%n1 ->] [%n2 ->]]"; simpl; eauto.
+Qed.
+
+Lemma LtOp_typed :
+  bin_op_typed LtOp TNat TNat TBool.
+Proof.
+  iIntros (v1 v2) "[[%n1 ->] [%n2 ->]]"; simpl; eauto.
+Qed.
+
+Lemma EqOp_Nat_typed :
+  bin_op_typed EqOp TNat TNat TBool.
+Proof.
+  iIntros (v1 v2) "[[%n1 ->] [%n2 ->]]"; simpl; eauto.
+Qed.
+
+Lemma EqOp_Bool_typed :
+  bin_op_typed EqOp TBool TBool TBool.
+Proof.
+  iIntros (v1 v2) "[[%b1 ->] [%b2 ->]]"; simpl; eauto.
+Qed.
 
 Lemma ctx_typed_app Gamma1 Gamma2 vs :
   ctx_typed (Gamma1 ++ Gamma2) vs |~
@@ -149,6 +185,10 @@ Tactic Notation "wp_absorb" constr(spat) :=
   iApply (absorb with spat);
     [apply wp_absorbing; intros; apply abs_absorbing | done |].
 
+(* ########################################################################## *)
+(** * Semantic typing rules *)
+(* ########################################################################## *)
+
 Lemma Unit_typed :
   val_typed VUnit TUnit.
 Proof.
@@ -177,6 +217,27 @@ Proof.
   iExists v; iFrame; StringMap.map_solver.
 Qed.
 
+Lemma Val_typed Gamma v A :
+  val_typed v A ->
+  typed Gamma (EVal v) A.
+Proof.
+  iIntros (Hv vs) "Hvs"; simpl.
+  iApply Val_wp. iSplitR; [| done]. by iApply Hv.
+Qed.
+
+Lemma Var_typed Gamma x A :
+  In (x, A) Gamma ->
+  typed Gamma (EVar x) A.
+Proof.
+  iIntros (HIn vs) "Hvs".
+  iInduction Gamma as [| [y B] Gamma] "IH" forall (vs); simpl in *; [done |].
+  destruct HIn as [? | HIn]; simplify_eq.
+  - iDestruct "Hvs" as "[(%v & -> & Hv) Hvs]".
+    iApply Val_wp. by iSplitL "Hv".
+  - iDestruct "Hvs" as "[? Hvs]".
+    wp_absorb "[- Hvs]". by iApply "IH".
+Qed.
+
 Lemma Lam_typed Gamma x e A1 A2 :
   ~In x (ctx_dom Gamma) ->
   typed ((x, A1) :: Gamma) e A2 ->
@@ -201,3 +262,351 @@ Proof.
   iApply (He2 with "Hvs2"); ex_done; iIntros (v2) "[Hv2 ?]".
   wp_absorb "[- Hv1 Hv2]". iApply ("Hv1" with "Hv2").
 Qed.
+
+Lemma Op_typed Gamma1 Gamma2 op e1 e2 A1 A2 B :
+  bin_op_typed op A1 A2 B ->
+  typed Gamma1 e1 A1 ->
+  typed Gamma2 e2 A2 ->
+  typed (Gamma1 ++ Gamma2) (EOp op e1 e2) B.
+Proof.
+  iIntros (Hop He1 He2 vs) "Hvs"; simpl.
+  iDestruct (ctx_typed_app with "Hvs") as "[Hvs1 Hvs2]".
+  iApply (He1 with "Hvs1"); ex_done; iIntros (v1) "[Hv1 ?]".
+  iApply (He2 with "Hvs2"); ex_done; iIntros (v2) "[Hv2 ?]".
+  iDestruct (Hop with "[$Hv1 $Hv2]") as (v Heval) "Hv".
+  iApply Op_wp. iFrame.
+Qed.
+
+Lemma Pair_typed Gamma1 Gamma2 e1 e2 A1 A2 :
+  typed Gamma1 e1 A1 ->
+  typed Gamma2 e2 A2 ->
+  typed (Gamma1 ++ Gamma2) (EPair e1 e2) (TProd A1 A2).
+Proof.
+  iIntros (He1 He2 vs) "Hvs"; simpl.
+  iDestruct (ctx_typed_app with "Hvs") as "[Hvs1 Hvs2]".
+  iApply (He1 with "Hvs1"); ex_done; iIntros (v1) "[Hv1 ?]".
+  iApply (He2 with "Hvs2"); ex_done; iIntros (v2) "[Hv2 ?]".
+  iApply Pair_wp. iSplitL "Hv1 Hv2"; [| done]. iExists v1, v2. by iFrame.
+Qed.
+
+Lemma LetPair_typed Gamma1 Gamma2 x1 x2 e1 e2 A1 A2 B :
+  ~In x1 (ctx_dom Gamma2) ->
+  ~In x2 (ctx_dom Gamma2) ->
+  x1 <> x2 ->
+  typed Gamma1 e1 (TProd A1 A2) ->
+  typed ((x1, A1) :: (x2, A2) :: Gamma2) e2 B ->
+  typed (Gamma1 ++ Gamma2) (ELetPair x1 x2 e1 e2) B.
+Proof. Admitted.
+
+Lemma If_typed Gamma1 Gamma2 e1 e2 e3 A :
+  typed Gamma1 e1 TBool ->
+  typed Gamma2 e2 A ->
+  typed Gamma2 e3 A ->
+  typed (Gamma1 ++ Gamma2) (EIf e1 e2 e3) A.
+Proof.
+  iIntros (He1 He2 He3 vs) "Hvs"; simpl.
+  iDestruct (ctx_typed_app with "Hvs") as "[Hvs1 Hvs2]".
+  iApply (He1 with "Hvs1"); ex_done; iIntros (v1) "[[%b ->] ?]". destruct b.
+  - iApply If_true_wp. wp_absorb "[- Hvs2]". by iApply He2.
+  - iApply If_false_wp. wp_absorb "[- Hvs2]". by iApply He3.
+Qed.
+
+Lemma Seq_typed Gamma1 Gamma2 e1 e2 A B :
+  typed Gamma1 e1 A ->
+  typed Gamma2 e2 B ->
+  typed (Gamma1 ++ Gamma2) (ESeq e1 e2) B.
+Proof.
+  iIntros (He1 He2 vs) "Hvs"; simpl.
+  iDestruct (ctx_typed_app with "Hvs") as "[Hvs1 Hvs2]".
+  iApply Seq_wp. iApply (He1 with "Hvs1"); ex_done; iIntros (v1) "[??]".
+  wp_absorb "[- Hvs2]". iApply (He2 with "Hvs2").
+Qed.
+
+Lemma Alloc_typed Gamma e A :
+  typed Gamma e A ->
+  typed Gamma (EAlloc e) (TRef A).
+Proof. Admitted.
+
+Lemma LinLoad_typed Gamma e A :
+  typed Gamma e (TRef A) ->
+  typed Gamma (ELinLoad e) (TProd (TRef TMoved) A).
+Proof. Admitted.
+
+Lemma LinLoad_copy_typed Gamma e A :
+  copy A ->
+  typed Gamma e (TRef A) ->
+  typed Gamma (ELinLoad e) (TProd (TRef A) A).
+Proof. Admitted.
+
+Lemma Store_typed Gamma1 Gamma2 e1 e2 A :
+  typed Gamma1 e1 (TRef A) ->
+  typed Gamma2 e2 A ->
+  typed (Gamma1 ++ Gamma2) (EStore e1 e2) (TRef A).
+Proof. Admitted.
+
+Lemma Free_typed Gamma e A :
+  typed Gamma e (TRef A) ->
+  typed Gamma (EFree e) A.
+Proof. Admitted.
+
+Lemma Throw_typed Gamma t e A :
+  typed Gamma e TNat ->
+  typed Gamma (EThrow t e) A.
+Proof. Admitted.
+
+Lemma Catch_typed Gamma1 Gamma2 e1 t e2 A :
+  typed Gamma1 e1 A ->
+  typed Gamma2 e2 (TFunOnce TNat A) ->
+  typed (Gamma1 ++ Gamma2) (ECatch e1 t e2) A.
+Proof. Admitted.
+
+Lemma Let_typed Gamma1 Gamma2 x e1 e2 A B :
+  ~In x (ctx_dom Gamma2) ->
+  typed Gamma1 e1 A ->
+  typed ((x, A) :: Gamma2) e2 B ->
+  typed (Gamma1 ++ Gamma2) (ELet x e1 e2) B.
+Proof. Admitted.
+
+Lemma InjL_typed Gamma e A1 A2 :
+  typed Gamma e A1 ->
+  typed Gamma (EInjL e) (TSum A1 A2).
+Proof. Admitted.
+
+Lemma InjR_typed Gamma e A1 A2 :
+  typed Gamma e A2 ->
+  typed Gamma (EInjR e) (TSum A1 A2).
+Proof. Admitted.
+
+Lemma Match_typed Gamma1 Gamma2 e x1 e1 x2 e2 A1 A2 B :
+  ~In x1 (ctx_dom Gamma2) ->
+  ~In x2 (ctx_dom Gamma2) ->
+  typed Gamma1 e (TSum A1 A2) ->
+  typed ((x1, A1) :: Gamma2) e1 B ->
+  typed ((x2, A2) :: Gamma2) e2 B ->
+  typed (Gamma1 ++ Gamma2) (EMatch e x1 e1 x2 e2) B.
+Proof. Admitted.
+
+Lemma copy_emp A v :
+  copy A ->
+  A v |~ EMP.
+Proof.
+  iIntros (HA) "Hv".
+  by iDestruct (HA with "Hv") as "Hv".
+Qed.
+
+Lemma copy_dup A v :
+  copy A ->
+  A v |~ A v ** A v.
+Proof.
+  iIntros (HA) "Hv".
+  iDestruct (HA with "Hv") as %Hv. iFrame "Hv". by iApply Hv.
+Qed.
+
+Lemma Moved_copy :
+  copy TMoved.
+Proof.
+  by iIntros (v) "_ !% _".
+Qed.
+
+Lemma Unit_copy :
+  copy TUnit.
+Proof.
+  by iIntros (v) "-> !% _".
+Qed.
+
+Lemma Nat_copy :
+  copy TNat.
+Proof.
+  iIntros (v) "[%n ->] !% _"; eauto.
+Qed.
+
+Lemma Bool_copy :
+  copy TBool.
+Proof.
+  iIntros (v) "[%b ->] !% _"; eauto.
+Qed.
+
+Lemma Prod_copy A1 A2 :
+  copy A1 ->
+  copy A2 ->
+  copy (TProd A1 A2).
+Proof.
+  iIntros (HA1 HA2 v) "(%w1 & %w2 & % & Hw1 & Hw2)".
+  iDestruct (HA1 with "Hw1") as "Hw1"; iDestruct "Hw1" as %Hw1.
+  iDestruct (HA2 with "Hw2") as "Hw2"; iDestruct "Hw2" as %Hw2.
+  iIntros "!% _"; iExists w1, w2. iSplitR; [done |].
+  iSplitR; [by iApply Hw1 | by iApply Hw2].
+Qed.
+
+Lemma Sum_copy A1 A2 :
+  copy A1 ->
+  copy A2 ->
+  copy (TSum A1 A2).
+Proof.
+  iIntros (HA1 HA2 v) "[%w [[% Hw] | [% Hw]]]".
+  - iDestruct (HA1 with "Hw") as "Hw"; iDestruct "Hw" as %Hw.
+    iIntros "!% _"; iExists w. iLeft; iSplitR; [done |]. by iApply Hw.
+  - iDestruct (HA2 with "Hw") as "Hw"; iDestruct "Hw" as %Hw.
+    iIntros "!% _"; iExists w. iRight; iSplitR; [done |]. by iApply Hw.
+Qed.
+
+Lemma Fun_copy A1 A2 :
+  copy (TFun A1 A2).
+Proof.
+  by iStartProof; iIntros (v) "%Hfun !% _".
+Qed.
+
+Lemma subty_refl A :
+  subty A A.
+Proof.
+  iIntros (v) "HA //".
+Qed.
+
+Lemma subty_trans A1 A2 A3 :
+  subty A1 A2 ->
+  subty A2 A3 ->
+  subty A1 A3.
+Proof.
+  iIntros (HA12 HA23 v) "HA1". iApply HA23. by iApply HA12.
+Qed.
+
+Lemma subty_copy A :
+  copy A ->
+  subty A TMoved.
+Proof.
+  iIntros (HA v) "Hv". by iApply copy_emp.
+Qed.
+
+Lemma Fun_to_FunOnce_subty A1 A2 :
+  subty (TFun A1 A2) (TFunOnce A1 A2).
+Proof.
+  iStartProof; iIntros (v Hfun w) "Hw". by iApply Hfun.
+Qed.
+
+Lemma Ref_subty A1 A2 :
+  subty A1 A2 ->
+  subty (TRef A1) (TRef A2).
+Proof.
+  iIntros (HA v) "(%l & %w & % & Hl & Hv)".
+  iExists l, w. iSplitR; [done |]; iFrame. by iApply HA.
+Qed.
+
+Lemma Prod_subty A1 A2 B1 B2 :
+  subty A1 A2 ->
+  subty B1 B2 ->
+  subty (TProd A1 B1) (TProd A2 B2).
+Proof.
+  iIntros (HA HB v) "(%w1 & %w2 & % & Hw1 & Hw2)".
+  iExists w1, w2. iSplitR; [done |].
+  iSplitL "Hw1"; [by iApply HA | by iApply HB].
+Qed.
+
+Lemma Sum_subty A1 A2 B1 B2 :
+  subty A1 A2 ->
+  subty B1 B2 ->
+  subty (TSum A1 B1) (TSum A2 B2).
+Proof.
+  iIntros (HA HB v) "[%w [[% Hw] | [% Hw]]]".
+  - iExists w. iLeft; iSplitR; [done |]. by iApply HA.
+  - iExists w. iRight; iSplitR; [done |]. by iApply HB.
+Qed.
+
+Lemma Fun_subty A1 A2 B1 B2 :
+  subty A2 A1 ->
+  subty B1 B2 ->
+  subty (TFun A1 B1) (TFun A2 B2).
+Proof. Admitted.
+
+Lemma FunOnce_subty A1 A2 B1 B2 :
+  subty A2 A1 ->
+  subty B1 B2 ->
+  subty (TFunOnce A1 B1) (TFunOnce A2 B2).
+Proof. Admitted.
+
+Lemma subctx_refl Gamma :
+  subctx Gamma Gamma.
+Proof.
+  iIntros (vs) "Hvs //".
+Qed.
+
+Lemma subctx_trans Gamma1 Gamma2 Gamma3 :
+  subctx Gamma1 Gamma2 ->
+  subctx Gamma2 Gamma3 ->
+  subctx Gamma1 Gamma3.
+Proof.
+  iIntros (HGamma12 HGamma23 vs) "Hvs". iApply HGamma23. by iApply HGamma12.
+Qed. 
+
+Lemma subctx_cons Gamma1 Gamma2 x A1 A2 :
+  subty A1 A2 ->
+  subctx Gamma1 Gamma2 ->
+  subctx ((x, A1) :: Gamma1) ((x, A2) :: Gamma2).
+Proof.
+  iIntros (HA HGamma vs) "Hvs"; simpl.
+  iDestruct "Hvs" as "[(%v & % & Hv) Hvs]".
+  iSplitR "Hvs"; [| by iApply HGamma].
+  iExists v; iSplitR; [done |]. by iApply HA.
+Qed.
+
+Lemma subctx_swap Gamma x1 x2 A1 A2 :
+  subctx ((x1, A1) :: (x2, A2) :: Gamma) ((x2, A2) :: (x1, A1) :: Gamma).
+Proof.
+  iIntros (vs) "Hvs"; simpl.
+  iDestruct "Hvs" as "((%v1 & % & Hv1) & (%v2 & % & Hv2) & Hvs)".
+  iFrame; iSplitL "Hv2"; eauto.
+Qed.
+
+Lemma subctx_copy_weakening Gamma x A :
+  copy A ->
+  subctx ((x, A) :: Gamma) Gamma.
+Proof.
+  iIntros (HA vs) "Hvs"; simpl.
+  iDestruct "Hvs" as "[(%v & _ & Hv) Hvs]".
+  iFrame. by iApply copy_emp.
+Qed.
+
+Lemma subctx_copy_contraction Gamma x A :
+  copy A ->
+  subctx ((x, A) :: Gamma) ((x, A) :: (x, A) :: Gamma).
+Proof.
+  iIntros (HA vs) "Hvs"; simpl.
+  iDestruct "Hvs" as "[(%v & % & Hv) Hvs]". iFrame.
+  iDestruct (copy_dup with "Hv") as "[Hv1 Hv2]"; [done |].
+  iSplitL "Hv1"; iExists v; by iFrame.
+Qed.
+
+Lemma val_subsumption v A1 A2 :
+  subty A1 A2 ->
+  val_typed v A1 ->
+  val_typed v A2.
+Proof.
+  iIntros (HA Hv) "_". iApply HA. by iApply Hv.
+Qed.
+
+Lemma subsumption Gamma1 Gamma2 e A1 A2 :
+  subctx Gamma2 Gamma1 ->
+  subty A1 A2 ->
+  typed Gamma1 e A1 ->
+  typed Gamma2 e A2.
+Proof.
+  iIntros (HGamma HA He vs) "Hvs".
+  iApply (He with "[Hvs]"); [by iApply HGamma |]; ex_done.
+  iIntros (v) "[Hv1 ?]". iSplitL "Hv1"; [| done]. by iApply HA.
+Qed.
+
+Definition terminates (e : expr) :Prop :=
+  exists r h, big_step e NatMap.empty r h.
+
+Section wp_adequacy.
+  Transparent sepEntails.
+
+  Lemma wp_adequacy phi ephi e :
+    (EMP |~ wp e (fun v => @[ phi v ]) (fun t v => @[ ephi t v ])) ->
+    exists r h, big_step e NatMap.empty r h /\ (phi # ephi) r.
+  Proof. Admitted.
+End wp_adequacy.
+
+Lemma type_soundness e A :
+  typed [] e A ->
+  terminates e.
+Proof. Admitted.
